Working on proof of liblinking

common/SmallstepLinkingLib.v
@@ -28,7 +28,7 @@ Section LINK'.
   Section WITH_SE.
     Context (se: Genv.symtbl).
 
-    Inductive frame :Type :=
+    Inductive frame : Type :=
     | caller:  Smallstep.state C -> frame
     | callee:  Smallstep.state A -> frame.
 
@@ -59,10 +59,10 @@ Section LINK'.
 
     Definition li := sum_li li1 li2.
 
-  (* Modeling the linking of "linked C program"(high level program) to asm program. The linked program will not have a C level outgoing interface anymore, because such linking with other C components have been done in the previous stage.  *)
     Inductive at_external: state -> query li -> Prop :=
       | at_external_intro_C s q k:
           Smallstep.at_external (C se) s q ->
+          valid_query (A se) q = false ->
           at_external (caller s :: k) (inl q)
       | at_external_intro_A s q k:
           Smallstep.at_external (A se) s q ->
@@ -117,6 +117,14 @@ Section LINK'.
 
               1.asm + lib.asm = out.asm                ->    A -->> A
 
+
+1. Why wrapper ?
+
+2. Diff mem model -> memory model transformation between the interface -> NMM works!
+
+3. Diff language C + IMP + + + + + + + + + + +
+
+4. Diff 
 *)
   (** * Properties *)
 
@@ -173,13 +181,137 @@ Section LINK'.
     determinate semantics_link_lib.
   Proof.
     intros HA HC se. unfold determinate in *.
-    Admitted.
+        constructor; cbn.
+    - destruct 1; inversion 1; subst_dep.
+      + edestruct (sd_determ (HC se) s t s' t2 s'0); intuition eauto; congruence.
+      + eelim sd_at_external_nostep. apply HC. all: eauto.
+      + edestruct (sd_determ (HA se) s t s' t2 s'0); intuition eauto; congruence.
+      + eelim sd_final_nostep; eauto.
+      + eelim sd_at_external_nostep. apply HC. all: eauto.
+      + destruct (sd_at_external_determ (HC se) s q q0); eauto.
+        destruct (sd_initial_determ (HA se) q s' s'0); eauto.
+        intuition auto. constructor.
+      + eelim sd_final_nostep; eauto.
+      + edestruct (sd_final_determ (HA se) s r r0); eauto.
+        edestruct (sd_after_external_determ (HC se) sk0 r s' s'0); eauto.
+        intuition auto. constructor.
+    - intros s t s' STEP. destruct STEP; cbn; eauto.
+      eapply sd_traces. 2: eauto. eauto.
+      eapply sd_traces. 2: eauto. eauto.
+    - destruct 1; inversion 1; subst.
+      edestruct (sd_initial_determ (HC se) q s s0); eauto.
+    - destruct 1.
+      + inversion 1; subst_dep.
+      eapply sd_at_external_nostep. 2: eauto. 2: eauto. eauto.
+      edestruct (sd_at_external_determ (HC se) s q q0); eauto. congruence.
+      + inversion 1; subst_dep.
+      eapply sd_at_external_nostep; eauto.
+      eapply sd_final_noext; eauto.
+    - destruct 1.
+      + inversion 1; subst_dep. f_equal.
+      eapply sd_at_external_determ; eauto.
+      + inversion 1; subst_dep. f_equal.
+      eapply sd_at_external_determ; eauto.
+    - destruct 1. inversion 1; subst_dep.
+      edestruct (sd_after_external_determ (HC se) s r s' s'0); eauto.
+      inversion 1; subst_dep.
+      edestruct (sd_after_external_determ (HA se) s r s' s'0); eauto.
+    - destruct 1. inversion 1; subst_dep.
+      + eapply sd_final_nostep. 2: eauto. 2: eauto. eauto.
+      + eapply sd_final_noext.  2: eauto. 2: eauto. eauto.
+    - destruct 1. inversion 1; subst_dep.
+      eapply sd_final_noext.  2: eauto. 2: eauto. eauto.
+    - destruct 1. inversion 1; subst_dep.
+      eapply sd_final_determ. apply HC. eauto. eauto.
+Qed.
 
 End LINK'.
 
+Section SUMCC.
+  Context {li1}{li1'}{li2}{li2'} (cc1: callconv li1 li1')(cc2: callconv li2 li2').
+
+  Definition li1_sum_li2 := sum_li li1 li2.
+  Definition li1'_sum_li2' := sum_li li1' li2'.
+
+  Definition ccworld_sum := sum (ccworld cc1) (ccworld cc2).
+  Definition match_senv_sum w se1 se2 : Prop :=
+    match w with
+      | inl w1 => match_senv cc1 w1 se1 se2
+      | inr w2 => match_senv cc2 w2 se1 se2
+    end.
+
+  Definition match_query_sum (w:ccworld_sum) (q1: query li1_sum_li2) (q2: query li1'_sum_li2') : Prop :=
+    match w,q1,q2 with
+      | inl w1, inl q11, inl q12 => match_query cc1 w1 q11 q12
+      | inr w2, inr q21, inr q22 => match_query cc2 w2 q21 q22
+      | _,_,_ => False
+    end.
+
+  Definition match_reply_sum (w:ccworld_sum) (r1: reply li1_sum_li2) (r2: reply li1'_sum_li2') : Prop :=
+    match w,r1,r2 with
+      | inl w1, inl r11, inl r12 => match_reply cc1 w1 r11 r12
+      | inr w2, inr r21, inr r22 => match_reply cc2 w2 r21 r22
+      | _,_,_ => False
+    end.
+
+  Program Definition sum_cc :=
+    mk_callconv _ _ ccworld_sum match_senv_sum match_query_sum match_reply_sum _ _.
+  Next Obligation.
+    destruct w; simpl in H; eapply match_senv_public_preserved; eauto.
+  Qed.
+  Next Obligation.
+    destruct w; simpl in H; eapply match_senv_valid_for; eauto.
+  Qed.
+
+(*  Program Definition sum_cc {li1_sum_li2}{li1'_sum_li2'}: callconv li1_sum_li2 li1'_sum_li2' :=
+    {|
+      ccworld := unit;
+      match_senv := match_senv;
+      match_query := match_query;
+      match_reply := match_reply;
+    |}.
+  Next Obligation. *)
+End SUMCC.
 
 Section FSIM.
+  Context {liC liA} (cc: callconv liC liA).
+
+  Context (C1 : Smallstep.semantics liC liC) (A : Smallstep.semantics liA liC).
+  Context (A1 : Smallstep.semantics liA liA) (A': Smallstep.semantics liA liA).
+  Context (H1 : fsim_components cc cc C1 A1) (H2: fsim_components cc_id cc A A').
+  Context (se1 se2: Genv.symtbl) (w: ccworld cc).
+  Context (Hse: match_senv cc w se1 se2).
+  Context (Hse1 : Genv.valid_for (skel C1) se1) (Hse2 : Genv.valid_for (skel C1) se2).
+
+  Definition index : Type := (fsim_index H1) + (fsim_index H2).
+
+  Inductive order : index -> index -> Prop :=
+    |order_l x y : fsim_order H1 x y -> order (inl x) (inl y)
+    |order_r x y : fsim_order H2 x y -> order (inr x) (inr y).
+
+  Inductive match_topframes w : index -> frame C1 A -> frame A1 A' -> Prop :=
+    |match_topframes_C s1 s2 idx:
+      match_senv cc w se1 se2 ->
+      Genv.valid_for (skel C1) se1 ->
+      fsim_match_states H1 se1 se2 w idx s1 s2 ->
+      match_topframes w (inl idx) (caller C1 A s1) (caller A1 A' s2)
+    |match_topframes_A s1 s2 idx:
+      match_senv cc w se1 se2 -> (*?????*)
+      Genv.valid_for (skel A) se1 ->
+      fsim_match_states H2 se1 se2 w idx s1 s2 ->
+      match_topframes w (inr idx) (callee C1 A s1) (callee A1 A' s2).
+
+
+  Variable match_states : index -> list (frame C1 A) -> list (frame A1 A') -> Prop.
+
+  Lemma semantics_simulation sk1 sk2:
+    fsim_properties (sum_cc cc cc_id) cc se1 se2 w
+      (semantics_link_lib C1 A sk1 se1)
+      (semantics_link_lib A1 A' sk2 se2)
+      index order match_states.
+    Admitted.
 End FSIM.
+
 
 Definition compose {li_C li_A}
            (C: Smallstep.semantics li_C li_C)
@@ -189,11 +321,25 @@ Definition compose {li_C li_A}
 Lemma compose_simulation {li_C li_A} (cc: callconv li_C li_A)
       (C1 : Smallstep.semantics li_C li_C) (A : Smallstep.semantics li_A li_C)
       (A1 : Smallstep.semantics li_A li_A) (A': Smallstep.semantics li_A li_A)
-      L1 L2:
+      (L1 : Smallstep.semantics (sum_li li_C li_A) li_C)
+      (L2 : Smallstep.semantics (sum_li li_A li_A) li_A):
   forward_simulation cc cc C1 A1 ->
-  forward_simulation cc cc A A' ->
+  forward_simulation cc_id cc A A' ->
   compose C1 A = Some L1 ->
   compose A1 A' = Some L2 ->
-  forward_simulation cc_id cc L1 L2.
+  forward_simulation (sum_cc cc cc_id) cc L1 L2.
 Proof.
+  intros [Ha] [Hb] H1 H2. unfold compose in *. unfold option_map in *.
+  destruct (link (skel C1) (skel A)) as [sk1|] eqn:Hsk1; try discriminate. inv H1.
+  destruct (link (skel A1) (skel A')) as [sk2|] eqn:Hsk2; try discriminate. inv H2.
+  constructor.
+(*  eapply Forward_simulation with (order cc L1 L2 HL) (match_states cc L1 L2 HL).
+  - destruct Ha, Hb. cbn. congruence.
+  - intros se1 se2 w Hse Hse1.
+    eapply semantics_simulation; eauto.
+    pose proof (link_linkorder _ _ _ Hsk1) as [Hsk1a Hsk1b].
+    intros [|]; cbn; eapply Genv.valid_for_linkorder; eauto.
+  - clear - HL. intros [i x].
+    induction (fsim_order_wf (HL i) x) as [x Hx IHx].
+    constructor. intros z Hxz. inv Hxz; subst_dep. eauto. *)
   Admitted.
